Add missing precondition in Sha wrapper + reprove old version

vale/code/arch/x64/interop/Sha_update_bytes_stdcall.fst
@@ -28,19 +28,26 @@ friend X64.Memory_s
 friend X64.Memory
 friend X64.Vale.Decls
 friend X64.Vale.StateLemmas
+friend LowStar.Monotonic.Buffer
 #set-options "--z3rlimit 60"
 
 open Vale_sha_update_bytes_stdcall
 
+#set-options "--initial_fuel 6 --max_fuel 6 --initial_ifuel 0 --max_ifuel 0"
+let create_buffer_list (ctx_b:s8) (in_b:s8) (k_b:s8) (stack_b:b8)  : (l:list b8{
+    l == [stack_b;ctx_b;in_b;k_b] /\
+  (forall x. {:pattern List.memP x l} List.memP x l <==> (x == ctx_b \/ x == in_b \/ x == k_b \/ x == stack_b))}) =
+  [stack_b;ctx_b;in_b;k_b]
 
-#set-options "--initial_fuel 6 --max_fuel 6 --initial_ifuel 2 --max_ifuel 2"
+#set-options "--max_fuel 0 --max_ifuel 0"
+
 let create_initial_trusted_state is_win ctx_b in_b num_val k_b stack_b (h0:HS.mem{pre_cond h0 ctx_b in_b num_val k_b /\ B.length stack_b == (if is_win then 264 else 104) /\ live h0 stack_b /\ buf_disjoint_from stack_b [ctx_b;in_b;k_b]}) : GTot TS.traceState =
   let taint_func (x:b8) : GTot taint =
     if StrongExcludedMiddle.strong_excluded_middle (x == ctx_b) then Secret else
     if StrongExcludedMiddle.strong_excluded_middle (x == in_b) then Secret else
     if StrongExcludedMiddle.strong_excluded_middle (x == k_b) then Secret else
     Public in
-  let buffers = stack_b::ctx_b::in_b::k_b::[] in
+  let buffers = create_buffer_list ctx_b in_b k_b stack_b in
   let (mem:mem) = {addrs = addrs; ptrs = buffers; hs = h0} in
   let addr_ctx_b = addrs ctx_b in
   let addr_in_b = addrs in_b in
@@ -62,7 +69,8 @@ let create_initial_trusted_state is_win ctx_b in_b num_val k_b stack_b (h0:HS.me
     | Rdx -> num_val
     | Rcx -> addr_k_b
     | _ -> init_regs r end)
-  in let xmms = init_xmms in
+  in let regs = FunctionalExtensionality.on reg regs
+  in let xmms = FunctionalExtensionality.on xmm init_xmms in
   let (s0:BS.state) = {BS.ok = true; BS.regs = regs; BS.xmms = xmms; BS.flags = 0;
        BS.mem = Interop.down_mem h0 addrs buffers} in
   {TS.state = s0; TS.trace = []; TS.memTaint = create_valid_memtaint mem buffers taint_func}
@@ -88,7 +96,7 @@ let create_initial_vale_state is_win ctx_b in_b num_val k_b stack_b (h0:HS.mem{p
     if StrongExcludedMiddle.strong_excluded_middle (x == in_b) then Secret else
     if StrongExcludedMiddle.strong_excluded_middle (x == k_b) then Secret else
     Public in
-  let buffers = stack_b::ctx_b::in_b::k_b::[] in
+  let buffers = create_buffer_list ctx_b in_b k_b stack_b in
   let (mem:mem) = {addrs = addrs; ptrs = buffers; hs = h0} in
   let addr_ctx_b = addrs ctx_b in
   let addr_in_b = addrs in_b in
@@ -110,7 +118,8 @@ let create_initial_vale_state is_win ctx_b in_b num_val k_b stack_b (h0:HS.mem{p
     | Rdx -> num_val
     | Rcx -> addr_k_b
     | _ -> init_regs r end)
-  in let xmms = init_xmms in
+  in let regs = X64.Vale.Regs.of_fun regs
+  in let xmms = X64.Vale.Xmms.of_fun init_xmms in
   {ok = true; regs = regs; xmms = xmms; flags = 0; mem = mem;
       memTaint = create_valid_memtaint mem buffers taint_func}
 
@@ -122,13 +131,11 @@ let create_lemma is_win ctx_b in_b num_val k_b stack_b (h0:HS.mem{pre_cond h0 ct
     assert (FunctionalExtensionality.feq (regs' s1.TS.state) (regs' s_init.TS.state));
     assert (FunctionalExtensionality.feq (xmms' s1.TS.state) (xmms' s_init.TS.state))
 
-
 let implies_pre_aux (b:s8) (n:nat64) : Lemma
   (requires length b == 64 `op_Multiply` n)
   (ensures buffer_length #(X64.Memory.TBase X64.Memory.TUInt128) b == 4 `op_Multiply` n) = 
-    length_t_eq (TBase TUInt128) b
+length_t_eq (TBase TUInt128) b
 
-// TODO: Prove these two lemmas if they are not proven automatically
 let implies_pre (is_win:bool) (h0:HS.mem) (ctx_b:s8) (in_b:s8) (num_val:nat64) (k_b:s8)  (stack_b:b8) : Lemma
   (requires pre_cond h0 ctx_b in_b num_val k_b /\ B.length stack_b == (if is_win then 264 else 104) /\ live h0 stack_b /\ buf_disjoint_from stack_b [ctx_b;in_b;k_b])
   (ensures (
@@ -174,8 +181,10 @@ let implies_post (is_win:bool) (va_s0:va_state) (va_sM:va_state) (va_fM:va_fuel)
     (buffer_as_seq #t va_s0.mem ctx_b));
   assert (Seq.equal
     (BV.as_seq va_sM.mem.hs ctx_b128)
-    (buffer_as_seq #t va_sM.mem ctx_b));   
+    (buffer_as_seq #t va_sM.mem ctx_b));     
   ()
+
+#set-options "--max_fuel 0 --initial_ifuel 1 --max_ifuel 1"
 
 let lemma_ghost_sha_update_bytes_stdcall is_win ctx_b in_b num_val k_b stack_b h0 =
   length_t_eq (TBase TUInt64) stack_b;
@@ -192,23 +201,31 @@ let lemma_ghost_sha_update_bytes_stdcall is_win ctx_b in_b num_val k_b stack_b h
   assert (state_eq_S s1 (state_to_S s_v));
   assert (FunctionalExtensionality.feq s1.TS.state.BS.regs (X64.Vale.Regs.to_fun s_v.regs));
   assert (FunctionalExtensionality.feq s1.TS.state.BS.xmms (X64.Vale.Xmms.to_fun s_v.xmms));
-  s1, f_v, s_v.mem.hs
+  assert (M.modifies (M.loc_union (M.loc_buffer stack_b) ( M.loc_buffer ctx_b)) h0 s_v.mem.hs);
+  (s1, f_v, s_v.mem.hs)
 
 #set-options "--max_fuel 0 --max_ifuel 0"
 
-let sha_update_bytes_stdcall ctx_b in_b num_val k_b  =
-  push_frame();
-  let (stack_b:b8) = B.alloca (UInt8.uint_to_t 0) (UInt32.uint_to_t (if win then 264 else 104)) in
- if win then
+irreducible
+let sha_update_bytes_stdcall_aux (ctx_b:s8) (in_b:s8) (num_val:nat64) (k_b:s8) (stack_b:b8) : Stack unit
+  (fun h -> pre_cond h ctx_b in_b num_val k_b  /\ B.length stack_b == (if win then 264 else 104) /\ live h stack_b /\ buf_disjoint_from stack_b [ctx_b;in_b;k_b])
+  (fun h0 _ h1 ->
+    post_cond h0 h1 ctx_b in_b num_val k_b  /\
+    M.modifies (M.loc_union (M.loc_buffer stack_b) ( M.loc_buffer ctx_b)) h0 h1) =
+  if win then
   st_put
     (fun h -> pre_cond h ctx_b in_b num_val k_b /\ B.length stack_b == 264 /\ live h stack_b /\ buf_disjoint_from stack_b [ctx_b;in_b;k_b])
     (fun h -> let _, _, h1 =
       lemma_ghost_sha_update_bytes_stdcall true ctx_b in_b num_val k_b stack_b h
-    in h1)
+    in (), h1)
   else st_put
     (fun h -> pre_cond h ctx_b in_b num_val k_b /\ B.length stack_b == 104 /\ live h stack_b /\ buf_disjoint_from stack_b [ctx_b;in_b;k_b])
     (fun h -> let _, _, h1 =
       lemma_ghost_sha_update_bytes_stdcall false ctx_b in_b num_val k_b stack_b h
-    in h1);
-  pop_frame()
+    in (), h1)
 
+let sha_update_bytes_stdcall ctx_b in_b num_val k_b  =
+  push_frame();
+  let (stack_b:b8) = B.alloca (UInt8.uint_to_t 0) (UInt32.uint_to_t (if win then 264 else 104)) in
+  sha_update_bytes_stdcall_aux ctx_b in_b num_val k_b stack_b;
+  pop_frame()
